SubroutineShare.v
@@ -7,155 +7,116 @@ Require Import Trace.
 Require Import Machine.
 Require Import ObsTrace.
 
-(* To add sharing, we extend our domain model to divide stack frames into addresses that
-   have been shared or passed.*)
 Section DOMAIN_MODEL.
 
-  (* Let's extend our previous example first with passing. Again we have a stack resulting
-     from caller A calling callee B, now with a value v as an argument. The stack looks like this:
-
-                     sp
-     -----------------------------------------------
-     | A's frame | v | Empty stack..................
-     -----------------------------------------------
-          a1      a2                a3
-
-     B has access to v and to everything above the stack pointer. But v is inaccessible!
-     We could treat it as part of B's frame, and therefore accessible, but that could
-     prove tricky with some calling conventions. Instead we label it "passed" and allow
-     it to be an exception to the inaccessibility rule.
-
-     Now suppose that B has an array whose address (a3) is taken. B calls a callee C.
-
-                                                 sp
-     --------------------------------------------------------
-     | A's frame | v | B's frame | arr | B again | Empty.....
-     --------------------------------------------------------
-          a1      a2               a3
-
-     From C's perspective, a2 is no longer passed - that represented access granted only
-     to the immediate callee, B. But a3 is "shared" because its address has been taken, and
-     possibly passed (we cannot statically prove that it was not in all cases, so we make no
-     guarantees.) It will remain shrared until deallocated on B's return. a1, finally, we term
-     "local," and its inaccessibility is respected by all callees.
-
-     Many systems provide some protection to shared data; the natural example
-     is a capability system, in which a shared object is accessible only
-     to a holder of a valid pointer, defined as one "descended" from the original.
-     Our machinery will not track anything as detailed as pointer provenance, and cannot
-     distinguish between legal and illegal uses of pointers to shared memory.
-
-     Instead, our protection properties apply only to components that have not been shared.
-     Once a component is shared, it is freely accessible, except in the narrow case of passed
-     variables. A variable is passed when its address is only taken by the immediate callee,
-     of its allocating function, and we assume that the compiler can guarantee that the pointer
-     does not escape. This is the case for stack-allocated argument passing between subroutines.
-     A passed component should be accessible in the immediate callee, then inaccessible in its
-     nested calls.
-   *)
-  
   Inductive ShareStatus :=
   | Local
-  | Shared
   | Passed
-  .
+  | Shared.
   
   Inductive StackDomain :=
-  | Inactive (sd:StackDomain) (ss:ShareStatus)
-  | Active (ss:ShareStatus)
+  | Claimed (d:nat)
+  | Unclaimed
   | Outside
   .
 
-  Definition statusOf sd :=
-    match sd with
-    | Inactive _ ss => Some ss
-    | Active ss => Some ss
-    | Outside => None
-    end.
-
-  (* Finally we need a way to map components to the domain they belong to. *)
-  Definition DomainMap := Component -> StackDomain.
+  (* All components belong to domain, and a domain map tells us which. *)
+  Definition DomainMap := Component -> (StackDomain * ShareStatus).
   
 End DOMAIN_MODEL.
 
 Section WITH_MAPS.
 
-  Variable cdm : CodeMap'.
-  Variable sm : Addr -> bool.
-  Variable pOf : MachineState -> PolicyState.
-  
-  Definition initD : DomainMap * nat :=
+  Variable cdm : CodeMap'. (* Map of where code lives in memory and its annotation. *)
+  Variable sm : Addr -> bool. (* Determines whether an address is in the stack. *)
+  Variable pOf : MachineState -> PolicyState. (* Policy initialization function. *)
+
+  (* We will use the machinery defined at the end of Machine.v to extend traces of the
+     machine with context that will inform our properties. In this case the context is a
+     pair of a Domain Map and a natural number representing the depth of the stack. *)
+
+  Definition context : Type := DomainMap * nat.
+
+  (* For the initial context, we construct a domain map that maps the stack to Accessible
+     and everything else to Outside. The stack depth is 0. *)
+  Definition initC : context :=
     let dm := fun k =>
                 match k with
                 | Mem a =>
                   if sm a
-                  then Active Local
-                  else Outside
-                | Reg r => Outside
+                  then (Unclaimed,Local)
+                  else (Outside,Shared)
+                | _ => (Outside,Shared)
                 end in
-    (dm,O).
+    (dm, O).
   
   (* Our update function checks an "annotation" on the code being executed.
      Annotations are defined in Machine.v as an alternative to a million different
-     maps, and the ones that matter are call, return, yield, and share.
+     maps, and the ones that matter here are call and return.
 
      Annotations are given by the compiler. We assume that the compiler can tell us
-     which instructions represent calls, returns, and yields. Shares are more complicated;
-     the compiler cannot directly tell us which component(s) are being shared, because sharing
-     is often dynamic. What it can do is identify a relation between the machine state
-     and the component(s) being shared.
-     
-     For an example, suppose that a caller is sharing an address as an argument to its callee.
-     It executes a store instruction that the compiler identifies as a share; the target of
-     the share is the address to which the argument is being stored, held within the appropriate
-     register. So, we would relate a given machine state to the contents of the register in that
-     state.
-     
-     This is a much stronger assumption of information from the compiler than we had before!
-     We now fully rely on the compiler to recognize returns, for instance. Relating returns
-     to the actual program state is the job of control flow property, WBCF.
-
-     Note that yields don't actually change the domain map, as they don't change which
-     addresses belong to which stacks. *)
-  
-  Definition updateD (m:MachineState) (prev:DomainMap*nat) : DomainMap * nat :=
+     which instructions represent calls and returns. *)
+  Definition updateC (m:MachineState) (prev:context) : context :=
     let '(dm, d) := prev in
     match AnnotationOf cdm (m (Reg PC)) with
+    | Some (share f) =>
+      let dm' := fun k =>
+                   match k with
+                   | Mem a =>
+                     match f m a, dm k with
+                     | Some true, (Unclaimed,Local) => (Unclaimed,Passed)
+                     | Some false, (Unclaimed,_) => (Unclaimed,Shared)
+                     | _, _ => dm k
+                     end
+                   | _ => dm k
+                   end in
+      (dm', d)
     | Some call => (* A call adjusts the domain map by marking the caller's frame "inactive" *)
                    (* and wrapping the remaining stack in a new instance of "active" *)
       let dm' := fun k =>
-                   match k, dm k with
-                   | _, Outside => Outside
-                   | Mem a, Active ss =>
-                     if wlt a (m (Reg SP))
-                     then Inactive (Active ss) ss
-                     else Active ss
-                   | Mem a, Inactive sd Passed =>
-                     Inactive (Inactive sd Passed) Local
-                   | Mem a, Inactive sd ss =>
-                     Inactive (Inactive sd ss) ss
-                   | _, _ => dm k
-                   end in
+                    match k, dm k with
+                    | _, (Outside,ss) => (Outside,ss)
+                    | Mem a, (Unclaimed,ss) =>
+                      if wlt a (m (Reg SP))
+                      then (Claimed d,ss)
+                      else (Unclaimed,Local)
+                    | _, _ => dm k
+                    end in
       (dm', d+1)
     | Some ret => (* A return unwraps the outermost domain of all components in the initial stack *)
       let dm' := fun k =>
-                   match dm k with
-                   | Inactive sd Passed => Active Local
-                   | Inactive sd ss => sd
-                   | _ => dm k
-                   end in
+                    match dm k with
+                    | (Claimed d', ss) =>
+                      if d =? d'
+                      then (Unclaimed,Local)
+                      else dm k
+                    | _ => dm k
+                    end in
       (dm', d-1)
-    | _ => (dm,d)
+    | _ => (dm, d)
     end.
 
-  Definition StackIntegrityUE : Prop :=
-    forall minit MCP k sd mcp mcp',
-      WithContextMP updateD initD (MPTraceOf (minit, pOf minit)) MCP ->
+  (* A component is inaccessible if it is claimed and local, or claimed by a
+     depth that is buried in the stack. *)
+  Definition Inaccessible (c:context) (k:Component) : Prop :=
+    exists d,
+      fst c k = (Claimed d, Local) \/
+      (fst c k = (Claimed d, Passed) /\ d < (snd c)-1).
+  
+  (* Now it's quite simple to define an "ultra eager" integrity property:
+     if we run from any initial state, updating the context as above, then
+     at any particular state where a component k is in an Inaccessible domain,
+     k has the same value in the following state (if any.) We term this property
+     ultra eager because it "checks" at each step that components that are inaccessible
+     don't change, the most frequent it is possible to check. *)
+  Definition SimpleStackIntegrityUE : Prop :=
+    forall minit MCP k mcp mcp',
+      WithContextMP updateC initC (MPTraceOf (minit, pOf minit)) MCP ->
       ContextSegment (fun _ _ => False) MCP (notfinished mcp (finished mcp')) ->
-      fst (cstate mcp) k = Inactive sd Local ->
+      Inaccessible (cstate mcp) k ->
       mstate mcp k = mstate mcp' k.
 
-    (* We can do a similar Ultra Eager style property with confidentiality, and since we're
+    (* We can do a similar ultra eager style property with confidentiality, and since we're
        not allowing sharing it is straightforward. But some preliminaries on confidentiality.
        Firstly: confidentiality is expressed in terms of "variant" states. A K-variant
        state of m is a state that agrees with m at every component not in the set K. It may also
@@ -171,44 +132,117 @@ Section WITH_MAPS.
     forall k,
       (m k <> m' k \/ n k <> n' k) ->
       m' k = n' k.
-  
-  Definition StackConfidentialityUE : Prop :=
-    forall minit MCP sd mcp mcp' n n' o,
-      WithContextMP updateD initD (MPTraceOf (minit, pOf minit)) MCP ->
-      ContextSegment (fun _ _ => False) MCP (notfinished mcp (finished mcp')) ->
-      variantOf (fun k => fst (cstate mcp) k = Inactive sd Local) (mstate mcp) n ->
-      step (mstate mcp) = (mstate mcp', o) ->
-      step n = (n',o) /\ sameDifference (mstate mcp) (mstate mcp') n n'.
 
-  Definition FindSegmentMP P mp dm MCP :=
+  (* Once again, we take adjacent pairs of states in the trace from an arbitrary
+     start state and check that a property holds between them. In this case, that
+     in any K-variant of the first state where K is the set of components that are
+     Inacessible in that state, the step has the same observable behavior and makes
+     the same changes to state. *)
+  Definition SimpleStackConfidentialityUE : Prop :=
+    forall minit MCP m dm d p m' dm' d' p' n o n' p'' o',
+      WithContextMP updateC initC (MPTraceOf (minit, pOf minit)) MCP ->
+      ContextSegment (fun _ _ => False) MCP (notfinished (m,(dm,d),p) (finished (m',(dm',d'),p'))) ->
+      variantOf (fun k => Inaccessible (dm,d) k) m n ->
+      mpstep (m,p) = Some (m',p',o) ->
+      mpstep (n,p) = Some (n',p'',o') ->
+      sameDifference m m' n n' /\ p = p'' /\ o = o'.
+
+  (* Once again, because this doesn't track initialization,
+     it doesn't actually fully work for the unclaimed memory. *)
+
+  (* Here are some helper relations to combine the addition of context to a trace,
+     and the segmenting of the resulting trace by a proposition P.*)
+  Definition FindSegmentMP P mp c MCP :=
     exists MCP',
-      WithContextMP updateD dm (MPTraceOf mp) MCP' /\
+      WithContextMP updateC c (MPTraceOf mp) MCP' /\
       ContextSegment P MCP' MCP.
 
-  Definition FindSegmentM P m dm MC :=
+  Definition FindSegmentM P m c MC :=
     exists MC',
-      WithContextM updateD dm (MTraceOf m) MC' /\
+      WithContextM updateC c (MTraceOf m) MC' /\
       ContextSegmentM P MC' MC.
+
+  (* For integrity, ultra eager properties are significantly stronger than we actually
+     need. In fact, we want to consider lazy policies that allow illegal writes at times
+     in the name of efficiency. So we should consider what our actual goal is here - what
+     use are these properties? Here is an example of how we might think of a program logic
+     call rule that lets us guarantee that from a call point, if execution returns to the
+     caller, Inaccessible components are preserved. *)
   
-  Definition StackIntegrityEager : Prop :=
-    forall minit MCP d k sd mcp mcp',
-      FindSegmentMP  (fun m c => snd c = d) (minit, pOf minit) initD MCP ->
+  Definition CallRule : Prop :=
+    forall minit MCP mcall dmcall dcall pcall,
+      WithContextMP updateC initC (MPTraceOf (minit, pOf minit)) MCP ->
+      InTrace (mcall,(dmcall,dcall),pcall) MCP ->
+      AnnotationOf cdm (mcall (Reg PC)) = Some call ->
+         (* Case 1: Divergence (including due to failstop) *)
+      (forall MCP' m' dm d p',
+          WithContextMP updateC (dmcall,dcall) (MPTraceOf (mcall,pcall)) MCP' ->
+          InTrace (m',(dm,d),p') MCP' ->
+          d > dcall)
+      \/ (* Case 2: Return *)
+      (exists mp o m' c' p' MCP',
+          mpstep (mcall,pcall) = Some (mp,o) /\
+          FindSegmentMP (fun m '(dm,d) => d > dcall) mp (updateC mcall (dmcall,dcall)) MCP' /\
+          Last MCP' (m',c',p') /\
+          forall a,
+            wlt a (mcall (Reg SP)) = true ->
+            mcall (Mem a) = m' (Mem a)).
+
+  (* We could use this as our ultimate specification, or just to guide our trace
+     properties. Note that this rule cares nothing for what happens to the state of
+     the Inaccessible components during the call, only that whe we return, they are
+     the same. Our eager property reflects this; instead of guaranteeing that they never
+     change, it guarantees that they are unchanged if and when the function returns. *)
+  
+  Definition SimpleStackIntegrityEager : Prop :=
+    forall minit MCP d k mcp mcp',
+      FindSegmentMP  (fun m c => snd c = d) (minit, pOf minit) initC MCP ->
       mcp = head MCP ->
-      fst (cstate mcp) k = Inactive sd Local ->
+      Inaccessible (cstate mcp) k ->
       Last MCP mcp' ->
       mstate mcp k = mstate mcp' k.
-  
-  Definition Stuck (MCP : @MCPTrace (DomainMap * nat)) : Prop :=
-    exists m c p,
-      Last MCP (m,c,p) ->
-      mpstep (m,p) = None.
 
-  Definition StackConfidentialityEager : Prop :=
-    forall minit M MO d sd m dm p n N NO,
+  Theorem EagerIntSufficient :
+    SimpleStackIntegrityEager ->
+    CallRule.
+  Proof.
+  Admitted.
+  
+  (* We can make a similar argument about confidentiality, though it may be odd to
+     think of a confidentiality call rule. We can at least think of the following as
+     the "caller's view" of confidentiality: that from the call to the return, its
+     Inaccessible memory ought change nothing about the observable behavior of the
+     machine, and if control returns, its Inaccessible memory also did not impact the
+     returned state. *)
+
+  Definition ConfRule : Prop :=
+    forall minit MCP mcall dmcall dcall pcall n MCP' N MO NO,
+      WithContextMP updateC initC (MPTraceOf (minit, pOf minit)) MCP ->
+      InTrace (mcall,(dmcall,dcall),pcall) MCP ->
+      AnnotationOf cdm (mcall (Reg PC)) = Some call ->
+      variantOf (fun k => Inaccessible (dmcall,dcall) k \/ fst (dmcall k) = Unclaimed) mcall n ->
+      (* Clause 1: output up to return identical *)
+      PrefixUpTo (fun '(_,(dm,d),_) => d = dcall) MCP MCP' ->
+      FindSegmentM (fun _ '(dm,d) => d = dcall) n (dmcall,dcall) N ->
+      ObsOfMCP MCP' MO ->
+      ObsOfMC N NO ->
+      ObsOfMP MO ~=_O ObsOfM NO /\
+      (* Clause 2: if return, then state changes the same *)
+      (forall m' dm' p',
+          Last MCP' (m',(dm',dcall),p') ->
+          exists n' dm'',
+            Last N (n',(dm'',dcall)) /\
+            sameDifference mcall m' n n').
+
+  (* The flip side of the caller's rule is the trace property that holds on subtraces
+     representing calls. This only needs to be strong enough to support the caller-side
+     reasoning, so here is an example of such an eager (but not ultra-eager) property. *)
+  Definition SimpleStackConfidentialityEager : Prop :=
+    forall minit M MO d m dm p n N NO,
       let P := (fun m c => snd c = d) in
-      FindSegmentMP P (minit, pOf minit) initD M ->
+      FindSegmentMP P (minit, pOf minit) initC M ->
       head M = (m,(dm,d),p) ->
-      variantOf (fun k => dm k = Inactive sd Local) m n ->
+      variantOf (fun k => Inaccessible (dm,d) k \/ fst (dm k) = Unclaimed) m n ->
       FindSegmentM P n (dm,d) N ->
       ObsOfMCP M MO ->
       ObsOfMC N NO ->
@@ -224,41 +258,117 @@ Section WITH_MAPS.
       (Infinite M ->
        ObsOfMP MO ~=_O ObsOfM NO)
       /\ (* Case 3 *)
-      (Stuck M ->
-       ObsOfMP MO <=_O ObsOfM NO).
+      (forall mend dmend pend,
+          Last M (mend, dmend, pend) ->
+          P mend (dm,d) ->
+          ObsOfMP MO <=_O ObsOfM NO).
 
-  Inductive StepsTo : MachineState -> MachineState -> Prop :=
-  | isNow : forall m, StepsTo m m
-  | stepsTo : forall m1 m2 m' o,
-      step m1 = (m',o) ->
-      StepsTo m' m2 ->
-      StepsTo m1 m2.
-
-  Definition CallRule : Prop :=
-    forall minit MCP mcall dmcall dcall pcall,
-      WithContextMP updateD initD (MPTraceOf (minit, pOf minit)) MCP ->
-      InTrace (mcall,(dmcall,dcall),pcall) MCP ->
-      AnnotationOf cdm (mcall (Reg PC)) = Some call ->
-         (* Case 1: Divergence (including due to failstop) *)
-      (forall MCP' m' dm d p',
-          WithContextMP updateD (dmcall,dcall) (MPTraceOf (mcall,pcall)) MCP' ->
-          InTrace (m',dm,p') MCP' ->
-          d > dcall)
-      \/ (* Case 2: Return *)
-      (exists m',
-          StepsTo mcall m' /\
-          (forall k sd,
-            dmcall k = Inactive sd Local ->
-            mcall k = m' k) /\
-          (forall n k,
-              variantOf (fun k' => exists sd, dmcall k = Inactive sd Local) mcall n ->
-              StepsTo n m')).
-
-  Theorem EagerSufficient :
-    StackIntegrityEager ->
-    StackConfidentialityEager ->
-    CallRule.
+  Theorem EagerConfSufficient :
+    SimpleStackConfidentialityEager ->
+    ConfRule.
   Proof.
   Admitted.
+
+  (* Now the above properties do a few things all at once that it helps to disentangle. They
+     quantify over all initial states, then over all segments of a trace at or above a certain
+     depth on the stack, ending with the return when the depth is reduced. And they state
+     properties of those segments. Lets focus on just capturing what it means for a trace
+     to respect the integrity and confidentiality of components, and separate out the finding
+     of the traces. The predicate K will indicate the set of components that must be protected. *)
+
+  Definition TraceIntegrityEager (K : Component -> Prop) (MCP:MCPTrace) : Prop :=
+    forall k (mcp':@MCPState context),
+      K k->
+      Last MCP mcp' ->
+      mstate (head MCP) k = mstate mcp' k.
+
+  (* The confidentiality trace property needs to know when the variant trace can be considered to have
+     returned, for which it takes a predicate on states and contexts, P. *)
+  Definition TraceConfidentialityEager (K : Component -> Prop)
+             (P:MachineState -> context -> Prop)
+             (MCP:@MCPTrace context) : Prop :=
+    forall MCP MO d m dm p n N NO,
+      head MCP = (m,(dm,d),p) ->
+      variantOf K m n ->
+      FindSegmentM P n (dm,d) N ->
+      ObsOfMCP MCP MO ->
+      ObsOfMC N NO ->
+         (* Case 1 *)
+      (forall mend dmend pend,
+          Last MCP (mend,dmend,pend) ->
+          ~ P mend (dm,d) ->
+          exists nend dnend,
+            Last N (nend,dnend) /\
+            ObsOfMP MO ~=_O ObsOfM NO /\
+            sameDifference m mend n nend)
+      /\ (* Case 2 *)
+      (Infinite MCP ->
+       ObsOfMP MO ~=_O ObsOfM NO)
+      /\ (* Case 3 *)
+      (forall mend dmend pend,
+          Last MCP (mend, dmend, pend) ->
+          P mend (dm,d) ->
+          ObsOfMP MO <=_O ObsOfM NO).
+
+  (* Now we can quantify over all initial states and segments starting with calls,
+     to create a property of the system that all calls enjoy both confidentiality and
+     integrity. *)
+  Definition StackSafety :=
+    forall minit MCP m dm d p,
+      let P := (fun m '(dm, d') => d' >= d) in
+      FindSegmentMP P (minit, pOf minit) initC MCP ->
+      head MCP = (m,(dm,d),p) ->
+      let K := (fun k => Inaccessible (dm,d) k) in
+      TraceIntegrityEager K MCP /\
+      TraceConfidentialityEager K P MCP.
+
+  Theorem StackSafetySufficient :
+    StackSafety ->
+    CallRule /\ ConfRule.
+  Proof.
+  Admitted.
+
+  (* ***** Control Flow Properties ***** *)
+  (* The addition of sharing does not change these. *)
+  
+  Definition ControlSeparation : Prop :=
+    forall minit m1 p1 m2 p2 o f1 f2 ann1 ann2,
+      InTrace (m1,p1) (MPTraceOf (minit, pOf minit)) ->
+      mpstep (m1,p1) = Some (m2, p2,o) ->
+      cdm (m1 (Reg PC)) = inFun f1 ann1 ->
+      cdm (m2 (Reg PC)) = inFun f2 ann2 ->
+      f1 <> f2 ->
+      AnnotationOf cdm (m1 (Reg PC)) = Some call \/
+      AnnotationOf cdm (m1 (Reg PC)) = Some ret \/
+      AnnotationOf cdm (m1 (Reg PC)) = Some yield.
+
+  Definition YieldBackIntegrity : Prop :=
+    forall mp mp1 mp2 MPout,
+      InTrace mp1 (MPTraceOf mp) ->
+      AnnotationOf cdm (ms mp1 (Reg PC)) = Some yield ->
+      SplitInclusive (fun mp2 => sm (ms mp1 (Reg PC)) = sm (ms mp (Reg PC))) (MPTraceOf mp) MPout (MPTraceOf mp2) ->
+      justRet (ms mp1) (ms mp2).
+
+  Definition ReturnIntegrity : Prop :=
+    forall d minit MCP m c p m' c' p',
+      FindSegmentMP (fun m '(dm,d') => d' >= d) (minit, pOf minit) initC MCP ->
+      head MCP = (m,c,p) ->
+      Last MCP (m',c',p') ->
+      justRet m m'.
+
+  Variable em:EntryMap.
+  
+  Definition EntryIntegrity : Prop :=
+  forall minit mp1 m2 p2 o,
+    InTrace mp1 (MPTraceOf (minit, pOf minit)) ->
+    mpstep mp1 = Some (m2,p2,o) ->
+    AnnotationOf cdm (ms mp1 (Reg PC)) = Some call ->
+    em (m2 (Reg PC)).
+
+  Definition WellBracketedControlFlow  : Prop :=
+    ControlSeparation /\
+    ReturnIntegrity /\
+    YieldBackIntegrity /\
+    EntryIntegrity.
 
 End WITH_MAPS.
